examples/Sek/PSek.ml
@@ -1,24 +1,24 @@
 open Weighted
 open PWSek
 
-type 'a psek = 'a pwsek
+type 'a psek = 'a swsek
 
-let psek_default = pwsek_default
+let psek_default = swsek_default
 
 let psek_create d =
-  pwsek_create d None
+  swsek_create d None
 
-let psek_is_empty = pwsek_is_empty
+let psek_is_empty = swsek_is_empty
 
 let psek_pop v s =
-  let s', x = pwsek_pop v None s in
+  let s', x = swsek_pop v None s in
   s', (unweighted x)
 
 let psek_push pov s x =
-  pwsek_push pov None s (mk_weighted x 1)
+  swsek_push pov None s (mk_weighted x 1)
 
 let psek_concat c0 c1 =
-  pwsek_concat None c0 c1
+  swsek_concat None c0 c1
 
 let psek_split c i =
-  pwsek_split None c i
+  swsek_split None c i
