examples/Sek/SWSek.ml
@@ -4,48 +4,48 @@ open View
 open Owner
 open SWChunk
 
-type 'a pwsek = { (* a sequence of ['a weighted] elements *)
+type 'a swsek = { (* a sequence of ['a weighted] elements *)
   p_sides : ('a swchunk) array; (* array of 2 items of type [(('a weighted) schunk) weighted] *)
-  p_mid : ('a partial_swchunk) pwsek option; (* a sequence of weighted chunks of weighted elements *)
+  p_mid : ('a partial_swchunk) swsek option; (* a sequence of weighted chunks of weighted elements *)
   p_weight : int
 }
 
 (*-----------------------------------------------------------------------------*)
 
-let pwsek_default s =
+let swsek_default s =
   swchunk_default s.p_sides.(0)
 
-let pwsek_create d oo =
+let swsek_create d oo =
   (* note: if oo = None, we could have pa0 for both sides *)
   let empty () = swchunk_create d oo in
   { p_sides = [| empty (); empty () |];
     p_mid = None;
     p_weight = 0 }
 
-let pwsek_is_empty s =
+let swsek_is_empty s =
   swchunk_is_empty s.p_sides.(0) &&
   swchunk_is_empty s.p_sides.(1)
 
 (*---------------------------------------------------------------------------*)
 
-(** [pwsek_extract_mid d mo] returns the middle sequence in the option [mo], if any,
+(** [swsek_extract_mid d mo] returns the middle sequence in the option [mo], if any,
    otherwise returns an empty middle sequence, built using the default value [d] *)
-let pwsek_extract_mid d oo mo =
+let swsek_extract_mid d oo mo =
   match mo with
-  | None -> pwsek_create (partial_swchunk_create d oo) oo
+  | None -> swsek_create (partial_swchunk_create d oo) oo
   | Some m -> m
   
-(** [pwsek_wrap_mid] takes a possibly empty middle sequence [m], and returns it
+(** [swsek_wrap_mid] takes a possibly empty middle sequence [m], and returns it
   as an option for storage in the [p_mid] record field. *)
-let pwsek_wrap_mid m =
-  if pwsek_is_empty m then
+let swsek_wrap_mid m =
+  if swsek_is_empty m then
     None
   else
     Some m
 
-(** [pwsek_mid_weight mo] returns the weight of the middle sek in option [mo], if any,
+(** [swsek_mid_weight mo] returns the weight of the middle sek in option [mo], if any,
   otherwise returns 0. *)
-let pwsek_mid_weight mo =
+let swsek_mid_weight mo =
   match mo with
   | None -> 0
   | Some m -> m.p_weight
@@ -55,21 +55,21 @@ let pwsek_mid_weight mo =
 (* Invariant: if one of the side is empty, then mid must be empty.
    Auxiliary functions*)
 
-let mk_pwsek_pov v front mid back w =
+let mk_swsek_pov v front mid back w =
   let front', back' = view_exchange v (front, back) in
   { p_sides = [| front'; back' |];
     p_mid = mid;
     p_weight = w }
 
 
-let mk_pwsek_pov_weight v front mid back =
-  let w = weight front + pwsek_mid_weight mid + weight back in
-  mk_pwsek_pov v front mid back w
+let mk_swsek_pov_weight v front mid back =
+  let w = weight front + swsek_mid_weight mid + weight back in
+  mk_swsek_pov v front mid back w
 
 (*-----------------------------------------------------------------------------*)
 (* Pop, which is needed to restore the invariant *)
 
-let rec pwsek_pop : 'a. view -> owner option -> 'a pwsek -> 'a pwsek * 'a weighted = fun v o s ->
+let rec swsek_pop : 'a. view -> owner option -> 'a swsek -> 'a swsek * 'a weighted = fun v o s ->
   let front, back = view_sides v s.p_sides in
   let mid = s.p_mid in
 
@@ -83,74 +83,74 @@ let rec pwsek_pop : 'a. view -> owner option -> 'a pwsek -> 'a pwsek * 'a weight
         match mid with
         | None -> x, front1, None, back
         | Some m ->
-          let m1, front2 = pwsek_pop v o m in
-          let m2 = pwsek_wrap_mid m1 in
+          let m1, front2 = swsek_pop v o m in
+          let m2 = swsek_wrap_mid m1 in
           x, front2, m2, back
       end else
         x, front1, mid, back
     end
   in
-  mk_pwsek_pov_weight v front' mid' back', x
+  mk_swsek_pov_weight v front' mid' back', x
   (* optimized as:
   let w = s.p_weight - weight x in
-  mk_pwsek_pov v front' mid' back' w, x *)
+  mk_swsek_pov v front' mid' back' w, x *)
 
 
 (*-----------------------------------------------------------------------------*)
 (* Auxiliary functions for invariant, continued *)
 
-let pwsek_populate v o s =
+let swsek_populate v o s =
   let front, back = view_sides v s.p_sides in
   if swchunk_is_empty front then begin
     match s.p_mid with
     | None -> s
     | Some m ->
-      let m1, front1 = pwsek_pop v o m in
-      let m2 = pwsek_wrap_mid m1 in
-      mk_pwsek_pov v front1 m2 back s.p_weight
+      let m1, front1 = swsek_pop v o m in
+      let m2 = swsek_wrap_mid m1 in
+      mk_swsek_pov v front1 m2 back s.p_weight
   end else
     s
 
-let pwsek_populate_both o s =
+let swsek_populate_both o s =
   (* Note: could take a view v as argument to decide which side to populate first *)
-  let s' = pwsek_populate Front o s in
-  pwsek_populate Back o s'
+  let s' = swsek_populate Front o s in
+  swsek_populate Back o s'
 
-let mk_pwsek_populated v o front mid back w =
-  let s = mk_pwsek_pov v front mid back w in
-  pwsek_populate_both o s
+let mk_swsek_populated v o front mid back w =
+  let s = mk_swsek_pov v front mid back w in
+  swsek_populate_both o s
 
-let mk_pwsek_weight_populated v o front mid back =
-  let s = mk_pwsek_pov_weight v front mid back in
-  pwsek_populate_both o s
+let mk_swsek_weight_populated v o front mid back =
+  let s = mk_swsek_pov_weight v front mid back in
+  swsek_populate_both o s
 
 (*-----------------------------------------------------------------------------*)
 (* Push *)
 
-let rec pwsek_push : 'a. view -> owner option -> 'a pwsek -> 'a weighted -> 'a pwsek = fun v o s x ->
-  let d = pwsek_default s in
+let rec swsek_push : 'a. view -> owner option -> 'a swsek -> 'a weighted -> 'a swsek = fun v o s x ->
+  let d = swsek_default s in
   let front, back = view_sides v s.p_sides in
   let mid = s.p_mid in
 
   let front1, mid1 =
     if swchunk_is_full front then begin
       let front' = swchunk_create d o in
-      let m = pwsek_extract_mid d o mid in
-      front', Some (pwsek_push v o m front)
+      let m = swsek_extract_mid d o mid in
+      front', Some (swsek_push v o m front)
 
-      (* TODO: would it be useful to define pwsek_push_into_mid v s c ? not so sure
-      let m = pwsek_extract_mid d s.p_mid in
-      Some (pwsek_push v m side)
+      (* TODO: would it be useful to define swsek_push_into_mid v s c ? not so sure
+      let m = swsek_extract_mid d s.p_mid in
+      Some (swsek_push v m side)
 
       code dessus devient
-      (swchunk_create d), (pwsek_push_into_mid v s front)
+      (swchunk_create d), (swsek_push_into_mid v s front)
       *)
     end else
       front, mid
     in
   let front2 = swchunk_push v o front1 x in
-  mk_pwsek_weight_populated v o front2 mid1 back
-  (* optimized as: mk_pwsek_populated v o front2 mid1 back (s.p_weight + weight x) *)
+  mk_swsek_weight_populated v o front2 mid1 back
+  (* optimized as: mk_swsek_populated v o front2 mid1 back (s.p_weight + weight x) *)
 
 
 (* LATER
@@ -171,55 +171,55 @@ let psek_peek pov s =
 (* push the chunk [c2] to the side of the middle sequence [s1] pointed by [v].
    If [c1] is the last chunk in the sequence [s1], we attempt to
    fuse the elements of [c2] into the back of [c1], if space allows. *)
-let pwsek_absorb v o s1 c2 =
+let swsek_absorb v o s1 c2 =
   if swchunk_is_empty c2 then
     s1
-  else if pwsek_is_empty s1 then
-    pwsek_push v o s1 c2
+  else if swsek_is_empty s1 then
+    swsek_push v o s1 c2
   else
-    let s1', c1 = pwsek_pop v o s1 in
+    let s1', c1 = swsek_pop v o s1 in
     if swchunk_size c1 + swchunk_size c2 <= capacity then begin
       let c12 = swchunk_concat o c1 c2 in
-      pwsek_push v o s1' c12
+      swsek_push v o s1' c12
     end else
-      pwsek_push v o s1 c2
+      swsek_push v o s1 c2
 
 (** given two middle sequences and a concatenation function with wanted spec,
   returns the middle *)
-let pwsek_merge_middle concat o mid1 mid2 =
+let swsek_merge_middle concat o mid1 mid2 =
   match mid1, mid2 with
   | None, _ -> mid2
   | _, None -> mid1
   | Some m1, Some m2 ->
-    let m2', c2 = pwsek_pop Front o m2 in
-    let m1' = pwsek_absorb Back o m1 c2 in
+    let m2', c2 = swsek_pop Front o m2 in
+    let m1' = swsek_absorb Back o m1 c2 in
     Some (concat o m1' m2')
 
-let rec pwsek_concat : 'a. owner option -> 'a pwsek -> 'a pwsek -> 'a pwsek = fun o s1 s2 ->
-  let d = pwsek_default s1 in
+let rec swsek_concat : 'a. owner option -> 'a swsek -> 'a swsek -> 'a swsek = fun o s1 s2 ->
+  let d = swsek_default s1 in
   let front1, back1 = view_sides Front s1.p_sides in
   let front2, back2 = view_sides Front s2.p_sides in
 
-  let m = pwsek_extract_mid d o s1.p_mid in
-  let mb1 = pwsek_absorb Back o m back1 in
-  let mb1f2 = pwsek_absorb Back o mb1 front2 in
-  let mid1 = pwsek_wrap_mid mb1f2 in
-  let mid = pwsek_merge_middle pwsek_concat o mid1 s2.p_mid in
+  let m = swsek_extract_mid d o s1.p_mid in
+  let mb1 = swsek_absorb Back o m back1 in
+  let mb1f2 = swsek_absorb Back o mb1 front2 in
+  let mid1 = swsek_wrap_mid mb1f2 in
+  let mid = swsek_merge_middle swsek_concat o mid1 s2.p_mid in
     
-  mk_pwsek_weight_populated Front o front1 mid back2
+  mk_swsek_weight_populated Front o front1 mid back2
   (* optimized as:
   let w = s1.p_weight + s2.p_weight in
-  mk_pwsek_populated Front o front1 mid back2 w *)
+  mk_swsek_populated Front o front1 mid back2 w *)
 
-(* [pwsek_split s w] returns [(s1, s2)] such that [s1 ++ s2 = s] and [s1] is
+(* [swsek_split s w] returns [(s1, s2)] such that [s1 ++ s2 = s] and [s1] is
   maximal such that [weight s1 <= w] *)
-let rec pwsek_split : 'a. owner option -> 'a pwsek -> int -> 'a pwsek * 'a pwsek = fun o s w ->
-  let d = pwsek_default s in
+let rec swsek_split : 'a. owner option -> 'a swsek -> int -> 'a swsek * 'a swsek = fun o s w ->
+  let d = swsek_default s in
   let front, back = view_sides Front s.p_sides in
   let mid = s.p_mid in
   let empty () = swchunk_create d o in
   let wf = weight front in
-  let wm = pwsek_mid_weight mid in
+  let wm = swsek_mid_weight mid in
 
   let front1, mid1, back1, front2, mid2, back2 =
     if w <= wf then
@@ -231,16 +231,16 @@ let rec pwsek_split : 'a. owner option -> 'a pwsek -> int -> 'a pwsek * 'a pwsek
         match mid with
         | None -> assert false (* Impossible as wm > 1 *)
         | Some m ->
-          let m1, m2 = pwsek_split o m w' in
-          let m2', f2 = pwsek_pop Front o m2 in (* non empty as m1.p_weight <= w - wf < wm so m2.p_weight > 0 *)
+          let m1, m2 = swsek_split o m w' in
+          let m2', f2 = swsek_pop Front o m2 in (* non empty as m1.p_weight <= w - wf < wm so m2.p_weight > 0 *)
           let b, f = swchunk_split o f2 (w' - m1.p_weight) in
-          front, pwsek_wrap_mid m1, b, f, pwsek_wrap_mid m2', back
+          front, swsek_wrap_mid m1, b, f, swsek_wrap_mid m2', back
       end else begin
         let b, f = swchunk_split o back (w' - wm) in
         front, mid, b, f, None, empty ()
       end
     end
   in
-  let s1 = mk_pwsek_weight_populated Front o front1 mid1 back1 in
-  let s2 = mk_pwsek_weight_populated Front o front2 mid2 back2 in
+  let s1 = mk_swsek_weight_populated Front o front1 mid1 back1 in
+  let s2 = mk_swsek_weight_populated Front o front2 mid2 back2 in
   s1, s2
